Batteries/Data/Fin/Basic.lean
@@ -107,19 +107,3 @@ protected def count (P : Fin n → Prop) [DecidablePred P] : Nat :=
 /-- Find the first true value of a decidable predicate on `Fin n`, if there is one. -/
 protected def find? (P : Fin n → Prop) [DecidablePred P] : Option (Fin n) :=
   foldr n (fun i v => if P i then some i else v) none
-
-/-- Custom recursor for `Fin (n+1)`. -/
-def recZeroSuccOn {motive : Fin (n+1) → Sort _} (x : Fin (n+1))
-    (zero : motive 0) (succ : (x : Fin n) → motive x.castSucc → motive x.succ) : motive x :=
-  match x with
-  | 0 => zero
-  | ⟨x+1, hx⟩ =>
-    let x : Fin n := ⟨x, Nat.lt_of_succ_lt_succ hx⟩
-    succ x <| recZeroSuccOn x.castSucc zero succ
-
-/-- Custom recursor for `Fin (n+1)`. -/
-def casesZeroSuccOn {motive : Fin (n+1) → Sort _} (x : Fin (n+1))
-    (zero : motive 0) (succ : (x : Fin n) → motive x.succ) : motive x :=
-  match x with
-  | 0 => zero
-  | ⟨x+1, hx⟩ => succ ⟨x, Nat.lt_of_succ_lt_succ hx⟩
